proof/refine/Invariants_H.thy
@@ -1,4 +1,5 @@
 (*
+ * Copyright 2023, Proofcraft Pty Ltd
  * Copyright 2020, Data61, CSIRO (ABN 41 687 119 230)
  *
  * SPDX-License-Identifier: GPL-2.0-only
@@ -22,6 +23,8 @@ arch_requalify_consts
   arch_valid_irq
   isArchFrameCap
   acapClass
+  valid_arch_badges
+  mdb_chunked_arch_assms
   global_refs'
   valid_arch_state'
   archMakeObjectT
@@ -211,10 +214,18 @@ definition live' :: "kernel_object \<Rightarrow> bool" where
   | KOArch ako          => hyp_live' ko"
 
 fun zobj_refs' :: "capability \<Rightarrow> obj_ref set" where
-  "zobj_refs' (EndpointCap r _ _ _ _ _)  = {r}"
-| "zobj_refs' (NotificationCap r _ _ _)  = {r}"
-| "zobj_refs' (ThreadCap r)              = {r}"
-| "zobj_refs' _                          = {}"
+  "zobj_refs' NullCap                        = {}"
+| "zobj_refs' DomainCap                      = {}"
+| "zobj_refs' (UntypedCap d r n f)           = {}"
+| "zobj_refs' (EndpointCap r badge x y z t)  = {r}"
+| "zobj_refs' (NotificationCap r badge x y)  = {r}"
+| "zobj_refs' (CNodeCap r b g gsz)           = {}"
+| "zobj_refs' (ThreadCap r)                  = {r}"
+| "zobj_refs' (Zombie r b n)                 = {}"
+| "zobj_refs' (ArchObjectCap ac)             = azobj_refs' ac"
+| "zobj_refs' (IRQControlCap)                = {}"
+| "zobj_refs' (IRQHandlerCap irq)            = {}"
+| "zobj_refs' (ReplyCap tcb m x)             = {}"
 
 definition ex_nonz_cap_to' :: "obj_ref \<Rightarrow> kernel_state \<Rightarrow> bool" where
   "ex_nonz_cap_to' ref \<equiv> \<lambda>s. \<exists>cref. cte_wp_at' (\<lambda>c. ref \<in> zobj_refs' (cteCap c)) cref s"
@@ -389,20 +400,13 @@ where
   \<forall>x \<in> dom (ksPSpace s). is_aligned x (objBitsKO (the (ksPSpace s x)))"
 
 definition
-  pspace_canonical' :: "kernel_state \<Rightarrow> bool"
-where
- "pspace_canonical' s \<equiv> \<forall>p \<in> dom (ksPSpace s). canonical_address p"
-
-definition
-  pspace_in_kernel_mappings' :: "kernel_state \<Rightarrow> bool"
-where
- "pspace_in_kernel_mappings' s \<equiv> \<forall>p \<in> dom (ksPSpace s). p \<in> kernel_mappings"
-
-definition
   pspace_distinct' :: "kernel_state \<Rightarrow> bool"
 where
   "pspace_distinct' s \<equiv>
    \<forall>x \<in> dom (ksPSpace s). ps_clear x (objBitsKO (the (ksPSpace s x))) s"
+
+definition pspace_canonical' :: "kernel_state \<Rightarrow> bool" where
+  "pspace_canonical' s \<equiv> \<forall>p \<in> dom (ksPSpace s). canonical_address p"
 
 definition
   valid_objs' :: "kernel_state \<Rightarrow> bool"
@@ -457,20 +461,21 @@ where
 
 definition
   "valid_badges m \<equiv>
-  \<forall>p p' cap node cap' node'.
-    m p = Some (CTE cap node) \<longrightarrow>
-    m p' = Some (CTE cap' node') \<longrightarrow>
-    (m \<turnstile> p \<leadsto> p') \<longrightarrow>
-    (sameRegionAs cap cap') \<longrightarrow>
-    (isEndpointCap cap \<longrightarrow>
-     capEPBadge cap \<noteq> capEPBadge cap' \<longrightarrow>
-     capEPBadge cap' \<noteq> 0 \<longrightarrow>
-     mdbFirstBadged node')
-    \<and>
-    (isNotificationCap cap \<longrightarrow>
-     capNtfnBadge cap \<noteq> capNtfnBadge cap' \<longrightarrow>
-     capNtfnBadge cap' \<noteq> 0 \<longrightarrow>
-     mdbFirstBadged node')"
+   \<forall>p p' cap node cap' node'.
+     m p = Some (CTE cap node) \<longrightarrow>
+     m p' = Some (CTE cap' node') \<longrightarrow>
+     m \<turnstile> p \<leadsto> p' \<longrightarrow>
+     (sameRegionAs cap cap' \<longrightarrow>
+       (isEndpointCap cap \<longrightarrow>
+        capEPBadge cap \<noteq> capEPBadge cap' \<longrightarrow>
+        capEPBadge cap' \<noteq> 0 \<longrightarrow>
+        mdbFirstBadged node')
+       \<and>
+       (isNotificationCap cap \<longrightarrow>
+        capNtfnBadge cap \<noteq> capNtfnBadge cap' \<longrightarrow>
+        capNtfnBadge cap' \<noteq> 0 \<longrightarrow>
+        mdbFirstBadged node'))
+     \<and> valid_arch_badges cap cap' node'"
 
 fun (sequential)
   untypedRange :: "capability \<Rightarrow> machine_word set"
@@ -542,6 +547,7 @@ definition
   m p = Some (CTE cap n) \<longrightarrow>
   m p' = Some (CTE cap' n') \<longrightarrow>
   sameRegionAs cap cap' \<longrightarrow>
+  mdb_chunked_arch_assms cap \<longrightarrow>
   p \<noteq> p' \<longrightarrow>
   (m \<turnstile> p \<leadsto>\<^sup>+ p' \<or> m \<turnstile> p' \<leadsto>\<^sup>+ p) \<and>
   (m \<turnstile> p \<leadsto>\<^sup>+ p' \<longrightarrow> is_chunk m cap p p') \<and>
@@ -851,8 +857,7 @@ definition valid_irq_handlers' :: "kernel_state \<Rightarrow> bool" where
                                  cap = IRQHandlerCap irq \<longrightarrow> irq_issued' irq s"
 
 definition
-  "irqs_masked' \<equiv> \<lambda>s. intStateIRQTable (ksInterruptState s) irqInvalid = IRQInactive \<and>
-                      (\<forall>irq > maxIRQ. intStateIRQTable (ksInterruptState s) irq = IRQInactive)"
+  "irqs_masked' \<equiv> \<lambda>s. \<forall>irq > maxIRQ. intStateIRQTable (ksInterruptState s) irq = IRQInactive"
 
 definition
   "valid_irq_masks' table masked \<equiv> \<forall>irq. table irq = IRQInactive \<longrightarrow> masked irq"
@@ -995,7 +1000,7 @@ abbreviation(input)
            \<and> valid_dom_schedule' s \<and> untyped_ranges_zero' s"
 
 lemma all_invs_but_sym_refs_not_ct_inQ_check':
-  "(all_invs_but_sym_refs_ct_not_inQ' and sym_refs \<circ> state_refs_of' and ct_not_inQ) = invs'"
+  "(all_invs_but_sym_refs_ct_not_inQ' and sym_refs \<circ> state_refs_of' and sym_refs \<circ> state_hyp_refs_of' and ct_not_inQ) = invs'"
   by (simp add: pred_conj_def conj_commute conj_left_commute invs'_def valid_state'_def)
 
 lemma all_invs_but_not_ct_inQ_check':
@@ -1344,9 +1349,36 @@ lemma sym_refs_bound_tcb_atD':
   apply auto
   done
 
+lemma state_hyp_refs_of'_elemD:
+  "\<lbrakk> ref \<in> state_hyp_refs_of' s x \<rbrakk> \<Longrightarrow> ko_wp_at' (\<lambda>obj. ref \<in> hyp_refs_of' obj) x s"
+  by (clarsimp simp add: state_hyp_refs_of'_def ko_wp_at'_def
+                  split: option.splits if_split_asm)
+
+lemma obj_at_state_hyp_refs_ofD':
+  "obj_at' P p s \<Longrightarrow> \<exists>ko. P ko \<and> state_hyp_refs_of' s p = hyp_refs_of' (injectKO ko)"
+  apply (clarsimp simp: obj_at'_real_def project_inject ko_wp_at'_def conj_commute)
+  apply (rule exI, erule conjI)
+  apply (clarsimp simp: state_hyp_refs_of'_def)
+  done
+
+lemma ko_at_state_hyp_refs_ofD':
+  "ko_at' ko p s \<Longrightarrow> state_hyp_refs_of' s p = hyp_refs_of' (injectKO ko)"
+  by (clarsimp dest!: obj_at_state_hyp_refs_ofD')
+
+lemma hyp_sym_refs_obj_atD':
+  "\<lbrakk> obj_at' P p s; sym_refs (state_hyp_refs_of' s) \<rbrakk> \<Longrightarrow>
+     \<exists>ko. P ko \<and> state_hyp_refs_of' s p = hyp_refs_of' (injectKO ko) \<and>
+        (\<forall>(x, tp)\<in>hyp_refs_of' (injectKO ko). ko_wp_at' (\<lambda>ko. (p, symreftype tp) \<in> hyp_refs_of' ko) x s)"
+  apply (drule obj_at_state_hyp_refs_ofD')
+  apply (erule exEI, clarsimp)
+  apply (drule sym, simp)
+  apply (drule(1) sym_refsD)
+  apply (erule state_hyp_refs_of'_elemD)
+  done
+
 lemma refs_of_live':
   "refs_of' ko \<noteq> {} \<Longrightarrow> live' ko"
-  apply (cases ko, simp_all)
+  apply (cases ko, simp_all add: live'_def)
     apply clarsimp
    apply (rename_tac notification)
    apply (case_tac "ntfnObj notification"; simp)
@@ -1418,8 +1450,8 @@ lemmas valid_irq_states'_def = valid_irq_masks'_def
 
 lemma valid_pspaceE' [elim]:
   "\<lbrakk>valid_pspace' s;
-    \<lbrakk> valid_objs' s; pspace_aligned' s; pspace_distinct' s; no_0_obj' s;
-      valid_mdb' s; pspace_canonical' s; pspace_in_kernel_mappings' s\<rbrakk> \<Longrightarrow> R \<rbrakk> \<Longrightarrow> R"
+    \<lbrakk> valid_objs' s; pspace_aligned' s; pspace_distinct' s; pspace_canonical' s; no_0_obj' s;
+      valid_mdb' s \<rbrakk> \<Longrightarrow> R \<rbrakk> \<Longrightarrow> R"
   unfolding valid_pspace'_def by simp
 
 lemma idle'_no_refs:
@@ -1577,7 +1609,7 @@ lemma state_hyp_refs_of'_pspaceI:
 
 lemma (in Invariants_H_pspaceI) valid_pspace':
   "valid_pspace' s \<Longrightarrow> ksPSpace s = ksPSpace s' \<Longrightarrow> valid_pspace' s'"
-  by  (auto simp add: valid_pspace'_def valid_objs'_def pspace_aligned'_def pspace_canonical'_def
+  by  (auto simp add: valid_pspace'_def valid_objs'_def pspace_aligned'_def
                      pspace_distinct'_def ps_clear_def no_0_obj'_def ko_wp_at'_def
                      typ_at'_def pspace_canonical'_def
            intro: valid_obj'_pspaceI valid_mdb'_pspaceI pspace_in_kernel_mappings'_pspaceI)
@@ -2251,17 +2283,13 @@ lemma pspace_aligned_update [iff]:
   "pspace_aligned' (f s) = pspace_aligned' s"
   by (simp add: pspace pspace_aligned'_def)
 
-lemma pspace_canonical_update [iff]:
-  "pspace_canonical' (f s) = pspace_canonical' s"
-  by (simp add: pspace pspace_canonical'_def)
-
-lemma pspace_in_kernel_mappings_update [iff]:
-  "pspace_in_kernel_mappings' (f s) = pspace_in_kernel_mappings' s"
-  by (simp add: pspace pspace_in_kernel_mappings'_def)
-
 lemma pspace_distinct_update [iff]:
   "pspace_distinct' (f s) = pspace_distinct' s"
   by (simp add: pspace pspace_distinct'_def ps_clear_def)
+
+lemma pspace_canonical_update [iff]:
+  "pspace_canonical' (f s) = pspace_canonical' s"
+  by (simp add: pspace pspace_canonical'_def ps_clear_def)
 
 lemma pred_tcb_at_update [iff]:
   "pred_tcb_at' proj P p (f s) = pred_tcb_at' proj P p s"
@@ -2537,7 +2565,7 @@ lemma class_linksD:
 
 lemma mdb_chunkedD:
   "\<lbrakk> m p = Some (CTE cap n); m p' = Some (CTE cap' n');
-     sameRegionAs cap cap'; p \<noteq> p'; mdb_chunked m \<rbrakk>
+     sameRegionAs cap cap'; p \<noteq> p'; mdb_chunked_arch_assms cap; mdb_chunked m \<rbrakk>
   \<Longrightarrow> (m \<turnstile> p \<leadsto>\<^sup>+ p' \<or> m \<turnstile> p' \<leadsto>\<^sup>+ p) \<and>
      (m \<turnstile> p \<leadsto>\<^sup>+ p' \<longrightarrow> is_chunk m cap p p') \<and>
      (m \<turnstile> p' \<leadsto>\<^sup>+ p \<longrightarrow> is_chunk m cap' p' p)"
@@ -2747,6 +2775,10 @@ lemma invs_sym' [elim!]:
   "invs' s \<Longrightarrow> sym_refs (state_refs_of' s)"
   by (simp add: invs'_def valid_state'_def)
 
+lemma invs_sym_hyp' [elim!]:
+  "invs' s \<Longrightarrow> sym_refs (state_hyp_refs_of' s)"
+  by (simp add: invs'_def valid_state'_def)
+
 lemma invs_sch_act_wf' [elim!]:
   "invs' s \<Longrightarrow> sch_act_wf (ksSchedulerAction s) s"
   by (simp add: invs'_def valid_state'_def)
@@ -2770,6 +2802,14 @@ lemma invs_valid_idle'[elim!]:
 lemma invs_valid_global'[elim!]:
   "invs' s \<Longrightarrow> valid_global_refs' s"
   by (fastforce simp: invs'_def valid_state'_def)
+
+lemma invs_pspace_canonical'[elim!]:
+  "invs' s \<Longrightarrow> pspace_canonical' s"
+  by (fastforce dest!: invs_valid_pspace' simp: valid_pspace'_def)
+
+lemma valid_pspace_canonical'[elim!]:
+  "valid_pspace' s \<Longrightarrow> pspace_canonical' s"
+  by (rule valid_pspaceE')
 
 lemma invs'_invs_no_cicd:
   "invs' s \<Longrightarrow> all_invs_but_ct_idle_or_in_cur_domain' s"
